Array.thy
@@ -2,29 +2,34 @@ theory Array
   imports Main
 begin
 
-type_synonym 'a array = "(nat \<Rightarrow> 'a) \<times> nat" 
+type_synonym 'a array = "nat \<Rightarrow> 'a" 
+
+definition interval :: "nat \<Rightarrow> nat \<Rightarrow> nat set" where
+  "interval k l \<equiv> {i. k \<le> i \<and> i \<le> l}"
 
 abbreviation array_length :: "'a array \<Rightarrow> nat" ("len _" [999] 1000) where
   "len a \<equiv> snd a"
-
-definition any_value :: "'a" where
-  "any_value \<equiv> SOME u. True"
 
 definition array_at :: "'a array \<Rightarrow> nat \<Rightarrow> 'a" (infixl "at" 100) where
   "a at i \<equiv> fst a i"
 
 definition array_update :: "'a array \<Rightarrow> nat \<Rightarrow> 'a \<Rightarrow> 'a array" where
-  "array_update a i n \<equiv> ((fst a)(i := n), snd a)"
+  "array_update a i n \<equiv> ((fst a) (i := n), snd a)"
 
-definition new_array :: "nat \<Rightarrow> 'a array" where
-  "new_array n \<equiv> (\<lambda>_. any_value, n)"
+fun array_fold :: "('a \<Rightarrow> 'b \<Rightarrow> 'b) \<Rightarrow> 'a array \<Rightarrow> 'b \<Rightarrow> 'b" where
+  "array_fold f (a, 0) = id"
+| "array_fold f (a, Suc n) = array_fold f (a, n) o f (a (Suc n))"
+
+fun array_foldl :: "('b \<Rightarrow> 'a \<Rightarrow> 'b) \<Rightarrow> 'b \<Rightarrow> 'a array \<Rightarrow> 'b" where
+  "array_foldl f b (a, 0) = b"
+| "array_foldl f b (a, Suc n) = array_foldl f (f b (a (Suc n))) (a, n)"
 
 primrec new_array_acc :: "'a list \<Rightarrow> (nat \<Rightarrow> 'a ) \<Rightarrow> nat \<Rightarrow> nat \<Rightarrow> 'a" where
   "new_array_acc (x#xs) f n = new_array_acc xs (f(n := x)) (Suc n)"
 | "new_array_acc [] f n = f"
 
 definition new_array_list :: "'a list \<Rightarrow> 'a array" where
-  "new_array_list xs \<equiv> (new_array_acc xs (\<lambda>_. any_value) 1, length xs + 1)"
+  "new_array_list xs \<equiv> (new_array_acc xs (\<lambda>_. SOME n. True) 1, length xs + 1)"
 
 fun sum_from_to :: "nat \<Rightarrow> nat \<Rightarrow> ('a :: {plus, zero}) array \<Rightarrow> 'a" where
   "sum_from_to i 0 a = 0"
@@ -33,9 +38,6 @@ fun sum_from_to :: "nat \<Rightarrow> nat \<Rightarrow> ('a :: {plus, zero}) arr
 definition sum :: "('a :: {plus, zero}) array \<Rightarrow> 'a" where
   "sum a \<equiv> sum_from_to 1 (len a) a"
 
-fun sorted_from_to :: "nat \<Rightarrow> nat \<Rightarrow> ('a :: order) array \<Rightarrow> bool" where
-  "sorted_from_to i 0 a \<longleftrightarrow> True"
-| "sorted_from_to i (Suc j) a \<longleftrightarrow> (if i \<le> Suc j then sorted_from_to i j a \<and> (a at j \<le> a at (Suc j)) else False)"
 
 value "sorted_from_to 2 4 (new_array_list [1, 2, 3 :: nat, 4, 5])"
 end
